c_examples/fig3b.c
@@ -6,6 +6,3 @@ int get() {return c;}
 
 void incr() { record(c); c++; }
 
-// int main(){
-//   return 0;
-// }
