driver/Clflags.ml
@@ -64,4 +64,5 @@ let option_timings = ref false
 let stdlib_path = ref Configuration.stdlib_path
 let use_standard_headers =  ref Configuration.has_standard_headers
 let option_reloc_elf = ref false
+let option_more_instr = ref false
 
